proofs/x86-64/avx2/ml_dsa_65/common/encoding/s2.ec
@@ -17,7 +17,11 @@ require import Array768 Array1536.
 
 require import Error_polynomial.
 
-import VecMat PolyLVec.
+import VecMat PolyLVec PolyKVec.
+
+op valid_s2_bytes (a : W8.t Array768.t) =
+    forall k, 0 <= k < kvec =>
+    valid_eta_bytes (Array128.init (fun i => a.[k * 128 + i])).
 
 lemma s2_encode _a :
     hoare [ M.s2____encode :
@@ -25,25 +29,30 @@ lemma s2_encode _a :
      ==>
        kvec_unflatten128 res =
            KArray.map (fun (p : poly) => Array128.of_list witness (BitPack p Eta Eta)) (lifts_wpolykvec (kvec_unflatten256 _a))
+       /\ valid_s2_bytes res
    ].
 have Eta_val := mldsa65_Eta.
 have Hkvec := mldsa65_kvec.
 proc => /=.
 while (0 <= i <= 6 /\ s2 = _a /\ wpolykvec_srng (kvec_unflatten256 _a) Eta Eta  /\
-       forall k, 0 <= k < i =>
+       (forall k, 0 <= k < i =>
        (kvec_unflatten128 encoded).[k] =
-       (map (fun (p : poly) => Array128.of_list witness (BitPack p Eta Eta)) (lifts_wpolykvec (kvec_unflatten256 _a))).[k]);
+       (map (fun (p : poly) => Array128.of_list witness (BitPack p Eta Eta)) (lifts_wpolykvec (kvec_unflatten256 _a))).[k]) /\
+       (forall k, 0 <= k < i =>
+       valid_eta_bytes (Array128.init (fun j => encoded.[k * 128 + j]))));
        last first.
-       + auto => /> &hr *;do split;1: smt().
-         move => r0 j0 *;rewrite tP => k kb; smt().
+       + auto => /> &hr *; do split; 1: smt().
+         + move => r0 j0 * Hfunc Hval; rewrite tP => k kb; smt().
+         + move => r0 j0 * Hfunc Hval k kb.
+           rewrite /valid_s2_bytes in Hval; exact (Hval k kb).
 wp; ecall (error_polynomial_encode (Array256.init (fun (i_0 : int) => _a.[i * 256 + i_0]))).
-auto => /> &hr ?? Hrng H ?;do split;1:smt().
+auto => /> &hr ?? Hrng H Hval ? [Hrr Heta]; do split; 1: smt().
 + move : Hrng; rewrite /wpolykvec_srng /wpoly_srng !allP /=  => Hrng ii iib.
   have := Hrng i{hr} _; 1:smt().
   rewrite allP /= /input_unflatten initiE 1:/# /= => Hrngj.
   have := Hrngj ii _; 1:smt().
   rewrite initiE 1:/# /= initiE 1:/# /= nth_sub 1:/# /#.
-move => ?? rr Hrr; do split;1,2: smt().
+move => ?? rr [Hrr Hval_rr]; do split; 1,2: smt().
 move => k kbl kbh.
 case(0<=k<i{hr}) => *.
 +
@@ -65,6 +74,24 @@ have -> : k = i{hr} by smt().
 
 rewrite initiE 1:/# /= tP => ii iib.
 rewrite  initiE 1:/# /= nth_sub 1:/# initiE 1:/# /= /#.
+move => k kbl kbh.
+case(0<=k<i{hr}) => *.
++ have -> : valid_eta_bytes
+    (Array128.init (fun j =>
+      (Array768.init (fun (i_0 : int) =>
+        if 128 * i{hr} <= i_0 < 128 * i{hr} + 128
+        then rr.[i_0 - 128 * i{hr}]
+        else encoded{hr}.[i_0])).[k * 128 + j])) =
+    valid_eta_bytes (Array128.init (fun j => encoded{hr}.[k * 128 + j])); last by smt().
+  congr; rewrite tP => j jb; rewrite !initiE 1:/# /=; smt().
+have -> : k = i{hr} by smt().
+have -> : Array128.init (fun j =>
+    (Array768.init (fun (i_0 : int) =>
+      if 128 * i{hr} <= i_0 < 128 * i{hr} + 128
+      then rr.[i_0 - 128 * i{hr}]
+      else encoded{hr}.[i_0])).[i{hr} * 128 + j]) = rr.
++ rewrite tP => j jb; rewrite !initiE 1:/# /=; smt().
+exact Hval_rr.
 qed.
 
 
@@ -82,48 +109,68 @@ lemma s2_encode_ph _a :
      ==>
        kvec_unflatten128 res =
            KArray.map (fun (p : poly) => Array128.of_list witness (BitPack p Eta Eta)) (lifts_wpolykvec (kvec_unflatten256 _a))
+       /\ valid_s2_bytes res
    ] = 1%r by conseq s2_encode_ll (s2_encode _a).
 
 
 lemma s2_decode _a :
     hoare [ M.s2____decode :
        encoded = _a
+       /\ valid_s2_bytes _a
      ==>
        lifts_wpolykvec (kvec_unflatten256 res) =
            KArray.map (fun (bytes : W8.t Array128.t) => BitUnpack (to_list bytes) Eta Eta) (kvec_unflatten128 _a)
+       /\ wpolykvec_srng (kvec_unflatten256 res) Eta Eta
    ].
 have Eta_val := mldsa65_Eta.
 have Hkvec := mldsa65_kvec.
 proc => /=.
-while (0 <= i <= 6 /\ encoded = _a /\
+while (0 <= i <= 6 /\ encoded = _a /\ valid_s2_bytes _a /\
        forall k, 0 <= k < i =>
        (lifts_wpolykvec (kvec_unflatten256 s2)).[k] =
-       (map (fun (bytes : W8.t Array128.t) => BitUnpack (to_list bytes) Eta Eta) (kvec_unflatten128 _a)).[k]);
+       (map (fun (bytes : W8.t Array128.t) => BitUnpack (to_list bytes) Eta Eta) (kvec_unflatten128 _a)).[k]
+       /\ wpoly_srng Eta Eta (kvec_unflatten256 s2).[k]);
        last first.
        + auto => /> &hr *; do split; 1: smt().
-         move => r0 j0 *; rewrite tP => k kb; smt().
+         move => r0 j0 * H; rewrite tP => k kb; smt().
 wp; ecall (error_polynomial_decode (Array128.init (fun (i_0 : int) => _a.[i * 128 + i_0]))).
-auto => /> &hr ??H?;split;1:smt().
-move => ? rr Hrr;do split;1,2:smt().
+auto => /> &hr ?? Hvalid H ? [Hrr Hrng]; do split; 1: smt().
++ (* valid_eta_bytes precondition for ecall *)
+  move => j jb; have := (Hvalid i{hr} _); 1: smt().
+  rewrite /valid_eta_bytes => Hv; have := Hv j jb.
+  congr; congr; rewrite initiE 1:/# /= /#.
+move => ? rr [Hrr Hrng]; do split; 1,2: smt().
 move => k kbl kbh.
 case(0<=k<i{hr}) => *.
-+ have -> : (lifts_wpolykvec
-   (kvec_unflatten256
++ split.
+  + have -> : (lifts_wpolykvec
+     (kvec_unflatten256
+        (Array1536.init
+           (fun (i_0 : int) => if i{hr} * n <= i_0 < i{hr} * n + n then rr.[i_0 - i{hr} * n] else s2{hr}.[i_0])))).[k] =
+      (lifts_wpolykvec (kvec_unflatten256 s2{hr})).[k]; last by smt().
+    rewrite !mapiE 1..2:/# initiE 1:/# /= initiE 1:/# /= tP =>  ii iib.
+    rewrite mapiE 1:/# /= initiE 1:/# /= mapiE 1:/# /= initiE 1:/# /= !nth_sub 1,2:/# initiE 1:/# /= /#.
+  + have -> : (kvec_unflatten256
       (Array1536.init
-         (fun (i_0 : int) => if i{hr} * n <= i_0 < i{hr} * n + n then rr.[i_0 - i{hr} * n] else s2{hr}.[i_0])))).[k] =
-    (lifts_wpolykvec (kvec_unflatten256 s2{hr})).[k]; last by smt().
-  rewrite !mapiE 1..2:/# initiE 1:/# /= initiE 1:/# /= tP =>  ii iib.
-  rewrite mapiE 1:/# /= initiE 1:/# /= mapiE 1:/# /= initiE 1:/# /= !nth_sub 1,2:/# initiE 1:/# /= /#.
+         (fun (i_0 : int) => if i{hr} * n <= i_0 < i{hr} * n + n then rr.[i_0 - i{hr} * n] else s2{hr}.[i_0]))).[k] =
+      (kvec_unflatten256 s2{hr}).[k]; last by smt().
+    rewrite initiE 1:/# /= tP => ii iib; rewrite initiE 1:/# /= nth_sub 1:/# initiE 1:/# /= /#.
 have -> : k = i{hr} by smt().
-+ have -> : (lifts_wpolykvec
-   (kvec_unflatten256
++ split.
+  + have -> : (lifts_wpolykvec
+     (kvec_unflatten256
+        (Array1536.init
+           (fun (i_0 : int) => if i{hr} * n <= i_0 < i{hr} * n + n then rr.[i_0 - i{hr} * n] else s2{hr}.[i_0])))).[i{hr}]  =
+      (lifts_wpoly rr); last first.
+    + rewrite Hrr mapiE 1:/# /=;congr;congr;rewrite /input_unflatten initiE 1:/# /= tP => ii iib.
+      by rewrite initiE 1:/# get_of_list 1:/# /= nth_sub /#.
+    rewrite mapiE 1:/# /= initiE 1:/# /= tP => ii iib.
+    rewrite !mapiE 1,2:/# /= initiE 1:/# /= nth_sub 1:/# initiE 1:/# /= /#.
+  + have -> : (kvec_unflatten256
       (Array1536.init
-         (fun (i_0 : int) => if i{hr} * n <= i_0 < i{hr} * n + n then rr.[i_0 - i{hr} * n] else s2{hr}.[i_0])))).[i{hr}]  =
-    (lifts_wpoly rr); last first.
-  + rewrite Hrr mapiE 1:/# /=;congr;congr;rewrite /input_unflatten initiE 1:/# /= tP => ii iib.
-    by rewrite initiE 1:/# get_of_list 1:/# /= nth_sub /#.
-rewrite mapiE 1:/# /= initiE 1:/# /= tP => ii iib.
-rewrite !mapiE 1,2:/# /= initiE 1:/# /= nth_sub 1:/# initiE 1:/# /= /#.
+         (fun (i_0 : int) => if i{hr} * n <= i_0 < i{hr} * n + n then rr.[i_0 - i{hr} * n] else s2{hr}.[i_0]))).[i{hr}] = rr.
+    + rewrite initiE 1:/# /= tP => ii iib; rewrite initiE 1:/# /= nth_sub 1:/# initiE 1:/# /= /#.
+    by exact Hrng.
 qed.
 
 lemma s2_decode_ll : islossless M.s2____decode.
@@ -138,7 +185,9 @@ qed.
 lemma s2_decode_ph _a :
     phoare [ M.s2____decode :
        encoded = _a
+       /\ valid_s2_bytes _a
      ==>
        lifts_wpolykvec (kvec_unflatten256 res) =
            KArray.map (fun (bytes : W8.t Array128.t) => BitUnpack (to_list bytes) Eta Eta) (kvec_unflatten128 _a)
+       /\ wpolykvec_srng (kvec_unflatten256 res) Eta Eta
    ] = 1%r by conseq s2_decode_ll (s2_decode _a).
